wip: proving loop-unrolling equivalence

examples/loop_equivalence/src/lib.rs
@@ -5,7 +5,21 @@ fn op(u: u64) -> u64 {
 }
 
 fn f<const N: usize>(mut arr: [u64; N]) -> [u64; N] {
+    #[cfg(hax)]
+    let _initial = arr.clone();
+
     for i in 0..N {
+        hax_lib::loop_invariant!(|i: usize| {
+            hax_lib::forall(|j: usize| {
+                if j < i {
+                    arr[j] == op(_initial[j])
+                } else if j < N {
+                    arr[j] == _initial[j]
+                } else {
+                    true
+                }
+            })
+        });
         arr[i] = op(arr[i]);
     }
     arr
@@ -18,7 +32,15 @@ fn g<const N: usize>(arr: &mut [u64; N]) {
 
     for i in 0..(N / 2) {
         hax_lib::loop_invariant!(|i: usize| {
-            arr[..2 * i] == f(*arr)[..2 * i] && arr[2 * i..] == _initial[2 * i..]
+            hax_lib::forall(|j: usize| {
+                if j < 2 * i {
+                    arr[j] == op(_initial[j])
+                } else if j < N {
+                    arr[j] == _initial[j]
+                } else {
+                    true
+                }
+            })
         });
         arr[2 * i] = op(arr[2 * i]);
         arr[2 * i + 1] = op(arr[2 * i + 1]);
