examples/loop_equivalence/proofs/lean/extraction/loop_equivalence_wip.lean
@@ -1,0 +1,246 @@
+
+-- Experimental lean backend for Hax
+-- The Hax prelude library can be found in hax/proof-libs/lean
+import Hax
+import Std.Tactic.Do
+import Std.Do.Triple
+import Std.Tactic.Do.Syntax
+open Std.Do
+open Std.Tactic
+
+set_option mvcgen.warning false
+set_option linter.unusedVariables false
+
+
+namespace loop_equivalence
+
+@[spec]
+def op (u : u64) : RustM u64 := do (u /? (2 : u64))
+
+def f (N : usize) (arr : (RustArray u64 N)) : RustM (RustArray u64 N) := do
+  let _initial : (RustArray u64 N) ←
+    (core_models.clone.Clone.clone (RustArray u64 N) arr);
+  let arr : (RustArray u64 N) ←
+    (rust_primitives.hax.folds.fold_range
+      (0 : usize)
+      N
+      (fun arr i =>
+        (do
+        (hax_lib.prop.constructors.forall
+          (fun j =>
+            (do
+            (hax_lib.prop.constructors.from_bool
+              (← if (← (j <? i)) then do
+                ((← arr[j]_?) ==? (← (op (← _initial[j]_?))))
+              else do
+                if (← (j <? N)) then do
+                  ((← arr[j]_?) ==? (← _initial[j]_?))
+                else do
+                  (pure true))) :
+            RustM hax_lib.prop.Prop))) :
+        RustM hax_lib.prop.Prop))
+      arr
+      (fun arr i =>
+        (do
+        let arr : (RustArray u64 N) ←
+          (rust_primitives.hax.monomorphized_update_at.update_at_usize
+            arr
+            i
+            (← (op (← arr[i]_?))));
+        (pure arr) :
+        RustM (RustArray u64 N))));
+  (pure arr)
+
+def g (N : usize) (arr : (RustArray u64 N)) : RustM (RustArray u64 N) := do
+  let _initial : (RustArray u64 N) ←
+    (core_models.clone.Clone.clone (RustArray u64 N) arr);
+  let arr : (RustArray u64 N) ←
+    (rust_primitives.hax.folds.fold_range
+      (0 : usize)
+      (← (N /? (2 : usize)))
+      (fun arr i =>
+        (do
+        (hax_lib.prop.constructors.forall
+          (fun j =>
+            (do
+            (hax_lib.prop.constructors.from_bool
+              (← if (← (j <? (← ((2 : usize) *? i)))) then do
+                ((← arr[j]_?) ==? (← (op (← _initial[j]_?))))
+              else do
+                if (← (j <? N)) then do
+                  ((← arr[j]_?) ==? (← _initial[j]_?))
+                else do
+                  (pure true))) :
+            RustM hax_lib.prop.Prop))) :
+        RustM hax_lib.prop.Prop))
+      arr
+      (fun arr i =>
+        (do
+        let arr : (RustArray u64 N) ←
+          (rust_primitives.hax.monomorphized_update_at.update_at_usize
+            arr
+            (← ((2 : usize) *? i))
+            (← (op (← arr[(← ((2 : usize) *? i))]_?))));
+        let arr : (RustArray u64 N) ←
+          (rust_primitives.hax.monomorphized_update_at.update_at_usize
+            arr
+            (← ((← ((2 : usize) *? i)) +? (1 : usize)))
+            (← (op (← arr[(← ((← ((2 : usize) *? i)) +? (1 : usize)))]_?))));
+        (pure arr) :
+        RustM (RustArray u64 N))));
+  let arr : (RustArray u64 N) ←
+    if (← ((← (N %? (2 : usize))) >? (0 : usize))) then do
+      (rust_primitives.hax.monomorphized_update_at.update_at_usize
+        arr
+        (← (N -? (1 : usize)))
+        (← (op (← arr[(← (N -? (1 : usize)))]_?))))
+    else do
+      (pure arr);
+  (pure arr)
+
+instance : BEq (RustArray u64 N) where
+  beq a b := (a.toVec = b.toVec)
+
+theorem triple_implies {f : RustM α} {Q : _ → _} {p} :
+  (⦃ ⌜ True ⌝ ⦄ f ⦃ ⇓?r =>  ⌜ Q r → p ⌝ ⦄) →
+  ((⦃ ⌜ True ⌝ ⦄ f ⦃ ⇓r =>  ⌜ Q r ⌝ ⦄) → p) := by sorry
+
+set_option hax_mvcgen.specset "int"
+set_option maxHeartbeats 1_000_000
+theorem g.spec (N : usize) (arr : (RustArray u64 N)) :
+    (do pure True : RustM _ ).holds →
+    ⦃ ⌜ True ⌝ ⦄ (g N arr) ⦃ ⇓
+       arr_future => ⌜
+         (do arr_future ==? (← (f N arr)): RustM _ ).holds ⌝ ⦄
+ := by
+   unfold RustM.holds
+   intro h_pre
+   hax_mvcgen [g] <;> (try grind [RustM.holds]) <;> unfold RustM.holds at *
+   · intros
+     mvcgen <;> try grind
+   · sorry -- integer overflow
+   · sorry -- integer overflow
+   · sorry -- integer overflow
+   · sorry -- integer overflow
+   · sorry -- integer overflow
+   · sorry -- integer overflow
+   · -- loop step in g
+     sorry
+   · -- post-condition if N % 2 > 0 (then-branch)
+     hax_mvcgen [f] <;> (try grind [RustM.holds]) <;> unfold RustM.holds at *
+
+     · -- [f] loop-invariant at the start of loop
+       intros
+       hax_mvcgen <;> (try grind [RustM.holds]) <;> unfold RustM.holds at *
+
+     · -- prove that f's loop invariant holds at i + 1 after the body
+       expose_names
+       intro j
+       hax_mvcgen <;> try grind
+       · -- j ≤ i
+         by_cases (j = i)
+         · subst_vars
+           rw [Vector.getElem_set_self]
+           rw [ ← UInt64.toNat_div,
+              UInt64.toNat_inj] at h_13
+           simp
+           apply triple_implies _ (h_11 j)
+           hax_mvcgen <;> try grind
+         · subst_vars
+           rw [Vector.getElem_set_ne] <;> try grind
+           apply triple_implies _ (h_11 j)
+           hax_mvcgen <;> try grind
+       · -- j > i
+         subst_vars
+         rw [Vector.getElem_set_ne] <;> try grind
+         apply triple_implies _ (h_11 j)
+         hax_mvcgen <;> try grind
+         -- j > N trivially true
+
+     · -- post-condition implied by [f] loop invariant at the end of the loop
+       expose_names
+       simp [BEq.beq]
+       ext i
+       apply triple_implies _ (h_9 (USize64.ofNat i)) <;> clear h_9
+       hax_mvcgen <;> try grind
+       · intro
+         apply triple_implies _ (h_1 (USize64.ofNat i)) <;> clear h_1
+         hax_mvcgen <;> try grind
+         · intro
+           subst_vars
+           rw [Vector.getElem_set]
+           split <;> try grind
+           · subst_vars
+             simp_all only [beq_iff_eq, USize64.toNat_inj]
+             rw [← USize64.toNat_sub_of_le] at * <;> try grind
+             expose_names
+             simp_all!
+             grind
+           · subst_vars
+             simp_all!
+             suffices (i = i % 18446744073709551616) by grind
+             grind
+         · have : (2*r + 1 = N) := by grind
+           simp_all only [decide_eq_true_iff.mp]
+           have : (i ≥ (N - 1).toNat) := by
+             simp
+             rw [ show (N-1) = 2*r by grind]
+             simp [decide_eq_false_iff_not.mp] at *
+             expose_names
+             have : 2 * r.toNat = 2 * r.toNat % 18446744073709551616 := by grind
+             rw [← this]
+             -- clearly true
+             sorry
+           have : (i = (N - 1).toNat) := by sorry
+           -- clearly true
+           sorry
+       · sorry -- i < N and i > N
+
+   · -- post-condition if N % 2 = 0 (else-branch)
+     hax_mvcgen [f] <;> (try grind [RustM.holds]) <;> unfold RustM.holds at *
+     · -- [f] loop-invariant at the start of loop
+       intros
+       hax_mvcgen <;> (try grind [RustM.holds]) <;> unfold RustM.holds at *
+     · -- prove that f's loop invariant holds at i + 1 after the body
+       expose_names
+       intro j
+       hax_mvcgen <;> try grind
+       · -- j ≤ i
+         by_cases (j = i)
+         · subst_vars
+           rw [Vector.getElem_set_self]
+           rw [ ← UInt64.toNat_div,
+              UInt64.toNat_inj] at h_8
+           simp
+           apply triple_implies _ (h_6 j)
+           hax_mvcgen <;> try grind
+         · subst_vars
+           rw [Vector.getElem_set_ne] <;> try grind
+           apply triple_implies _ (h_6 j)
+           hax_mvcgen <;> try grind
+       · -- j > i
+         subst_vars
+         rw [Vector.getElem_set_ne] <;> try grind
+         apply triple_implies _ (h_6 j)
+         hax_mvcgen <;> try grind
+         -- j > N trivially true
+     · -- post-condition implied by [f] loop invariant at the end of the loop
+       expose_names
+       suffices r_1 = r_3 by
+         rw [this]
+         simp [BEq.beq]
+       cases r_1
+       cases r_3
+       expose_names
+       suffices toVec = toVec_1 by grind
+       ext i
+       apply triple_implies _ (h_4 (USize64.ofNat i))
+       hax_mvcgen <;> try grind
+       · intro
+         apply triple_implies _ (h_1 (USize64.ofNat i))
+         hax_mvcgen <;> try grind
+         intro
+         subst_vars
+         simp_all
+         grind
+       · sorry -- i < N and i > N
